\documentclass[12pt, letterpaper]{memoir}
\usepackage{MyStyle}
\newgeometry{hmargin=.85in,vmargin=0.65in}

\begin{document}
\newpage
\pagestyle{empty}

~
\vspace{-3em}
\begin{center}
	{\LARGE 3610 Final Exam Equations and Constants}
\end{center}

\vspace{-1em}\noindent
\begin{minipage}{0.57\linewidth}
	\begin{mdframed}
		\begin{tabular}{rlcrl}
			\multicolumn{5}{c}{Gas Constant Values}                                       \\ \midrule
			$8.314$   & $\dfrac{J}{mole~K}$     &  & $0.08314$ & $\dfrac{L~bar}{mole~K}$  \\ \\
			$0.08206$ & $\dfrac{L~atm}{mole~K}$ &  & $8.314$   & $\dfrac{m^3~Pa}{mole~K}$ \\ \\
		\end{tabular}
		\begin{tabular}{rlcrl}
			\multicolumn{5}{c}{Boltzmann Constant Values}                                 \\ \midrule
			$1.381 \times 10^{-23}$ & $\dfrac{J}{K}$ &  & $0.6950$ & $\dfrac{cm^{-1}}{K}$ \\ \\
		\end{tabular}
	\end{mdframed}
\end{minipage}
\hspace{20pt}
\begin{minipage}{0.4\linewidth}
	\begin{mdframed}
		\begin{tabular}{rcl}
			\multicolumn{3}{c}{Conversions}  \\ \midrule
			$1~L~atm $ & $=$ & $101.325~J$   \\ \\
			$1~atm $   & $=$ & $1.01325~bar$ \\ \\
			$1~atm $   & $=$ & $760~torr$    \\ \\
			$1~atm $   & $=$ & $101,325~Pa$  \\ \\
		\end{tabular}
	\end{mdframed}
\end{minipage}

\begin{equation*}
	F=96,485\frac{C}{mol} \hspace{14em} e=1.60217662\times10^{-19} C
\end{equation*}


\noindent
\begin{minipage}{0.5\linewidth}
	\begin{equation*}
		H = U + pV
	\end{equation*}

	\begin{equation*}
		\mathrm{d} U = \dbar q + \dbar w
	\end{equation*}

	\begin{equation*}
		\dbar w = -p_{external} \mathrm{d}V
	\end{equation*}

	\begin{equation*}
		p = \frac{nRT}{V-nb} - a\frac{n^2}{V^2}
	\end{equation*}

	\begin{equation*}
		v_{rms} = \left(\frac{3RT}{M}\right)^{\nicefrac{1}{2}}
	\end{equation*}

	\begin{equation*}
		\Delta U_V = C_V~\Delta T
	\end{equation*}

	\begin{equation*}
		z = \sigma v_{rel}\mathcal{N}
	\end{equation*}



\end{minipage}
\begin{minipage}{0.5\linewidth}
	\begin{equation*}
		Z=\dfrac{pV}{nRT}=\left(1+\dfrac{B}{V_m} + \dfrac{C}{V_m^2}+\ldots\right)
	\end{equation*}

	\begin{equation*}
		C_{V,m} = \dfrac{1}{2}R\cdot n_{D.o.F}
	\end{equation*}

	\begin{equation*}
		C_{p,m} = C_{V,m}+R
	\end{equation*}

	\begin{equation*}
		v_{mean} = \left(\frac{8RT}{\pi M}\right)^{\nicefrac{1}{2}}
	\end{equation*}

	\begin{equation*}
		\Delta H_p= C_p~\Delta T
	\end{equation*}

	\begin{equation*}
		pV=nRT
	\end{equation*}

	\begin{equation*}
		v_{rel} = \sqrt{2}v_{mean}
	\end{equation*}




\end{minipage}

\noindent
\begin{minipage}{0.5\linewidth}
	\begin{equation*}
		\mathcal{N} = \frac{N}{V}=\frac{p}{k_BT}
	\end{equation*}

	\begin{equation*}
		\Delta H_{rxn}(T_2) = \Delta H_{rxn}(T_1) + \int_{T_1}^{T_2} \! \Delta C_{p}\mathrm{d}T
	\end{equation*}

	\begin{equation*}
		\Delta H^\circ_{rxn} = \sum\limits_{products} \nu_i\Delta H^\circ_{f,i} - \sum\limits_{reactants} \nu_j\Delta H^\circ_{f,j}
	\end{equation*}

	\begin{equation*}
		p_iV_i^\gamma = p_fV_f^\gamma \hspace{4em} \gamma = \dfrac{C_{p,m}}{C_{V,m}}
	\end{equation*}

	\begin{equation*}
		V_iT_i^c=V_fT_f^c \hspace{4em} c=\dfrac{C_{V,m}}{R}
	\end{equation*}
\end{minipage}
\begin{minipage}{0.5\linewidth}
	\begin{equation*}
		\lambda = \dfrac{v_{rel}}{z}=\frac{k_BT}{\sigma p}
	\end{equation*}

	\begin{equation*}
		\Delta H \approx \Delta U + \Delta n_{gas}RT
	\end{equation*}

	\begin{equation*}
		\pi_T=\left(\frac{\partial U}{\partial V}\right)_{\!\!T}
	\end{equation*}

	\begin{equation*}
		\alpha=\frac{1}{V}\left(\dfrac{\partial V}{\partial T}\right)_{\!\!p}
	\end{equation*}

	\begin{equation*}
		\kappa_T=-\frac{1}{V}\left(\dfrac{\partial V}{\partial p}\right)_{\!\!T}
	\end{equation*}
\end{minipage}

\begin{equation*}
	\mathrm{d}U=\left(\dfrac{\partial U}{\partial V}\right)_{\!\!T}\mathrm{d}V + \left(\dfrac{\partial U}{\partial T}\right)_{\!\!V}\mathrm{d}T=\pi_T\mathrm{d}V + C_V\mathrm{d}T
\end{equation*}

\begin{equation*}
	\mathrm{d}H=\left(\dfrac{\partial H}{\partial p}\right)_{\!\!T}\mathrm{d}p + \left(\dfrac{\partial H}{\partial T}\right)_{\!\!p}\mathrm{d}T=-\mu C_p{d}p + C_p\mathrm{d}T
\end{equation*}

\noindent
\begin{minipage}{0.5\linewidth}
	\begin{equation*}
		G = H-TS
	\end{equation*}

	\begin{equation*}
		\mathrm{d}G=-S\mathrm{d}T+V\mathrm{d}p
	\end{equation*}

	\begin{equation*}
		S=k_B\ln \mathcal{W}
	\end{equation*}

	\begin{equation*}
		\dfrac{q_H}{q_C}=-\dfrac{T_H}{T_C}
	\end{equation*}

	\begin{equation*}
		\eta = \dfrac{w}{q_H}
	\end{equation*}
\end{minipage}
\begin{minipage}{0.5\linewidth}
	\begin{equation*}
		A = U-TS
	\end{equation*}

	\begin{equation*}
		\left(\dfrac{\partial \nicefrac{\Delta G}{T}}{\partial T}\right)_p=-\dfrac{\Delta H}{T^2}
	\end{equation*}

	\begin{equation*}
		C_V = \dfrac{1}{2}R\cdot n_{D.o.F}
	\end{equation*}

	\begin{equation*}
		C_p = C_V+R
	\end{equation*}

	\begin{equation*}
		\mathrm{d} S_{system} = \dfrac{~\dbar q_{reversible}}{T}
	\end{equation*}
\end{minipage}

\begin{equation*}
	S(T)=S(0)+\int_0^T\dfrac{C_p}{T}\mathrm{d}T+\sum\limits_{transitions}\dfrac{\Delta H_{trs}}{T_{trs}}
\end{equation*}

\begin{equation*}
	\ln\dfrac{p_2}{p_1}=\dfrac{-\Delta H}{R}\left(\dfrac{1}{T_2}-\dfrac{1}{T_1}\right)
\end{equation*}

\noindent
\begin{minipage}[t]{0.5\linewidth}


	\begin{equation*}
		\eta = 1 - \dfrac{T_C}{T_H}
	\end{equation*}

	\begin{equation*}
		\Delta S_T=nR\ln\dfrac{V_f}{V_i}
	\end{equation*}

	\begin{equation*}
		\Delta S_p=C_p\ln\dfrac{T_f}{T_i}
	\end{equation*}

	\begin{equation*}
		G(p_2) = G(p_1)+nRT\ln\dfrac{p_2}{p_1}
	\end{equation*}

	\begin{equation*}
		\Delta S(T_2) = \Delta S(T_1) + \int_{T_1}^{T_2} \! \dfrac{\Delta C_{p}}{T}\mathrm{d}T
	\end{equation*}

	\begin{equation*}
		\dfrac{\mathrm{d}p}{\mathrm{d}T}=\dfrac{\Delta H}{T\Delta V_m}
	\end{equation*}

	\begin{equation*}
		\Delta G_{mix} = nRT\left(\chi_A\ln\chi_A+\chi_B\ln\chi_B\right)
	\end{equation*}

	\begin{equation*}
		p_A=\chi_Ap^{\star}_A
	\end{equation*}

	\begin{equation*}
		\mu_A=\mu_A^{\star}+RT\ln\chi_A
	\end{equation*}



\end{minipage}
\begin{minipage}[t]{0.5\linewidth}
	\begin{equation*}
		\mathrm{d} S_{surrounding} = -\dfrac{~\dbar q_{sys}}{T}
	\end{equation*}

	\begin{equation*}
		\Delta S_V=C_V\ln\dfrac{T_f}{T_i}
	\end{equation*}

	\begin{equation*}
		\Delta S_{trs}=\dfrac{\Delta H_{trs}}{T}
	\end{equation*}

	\begin{equation*}
		F=C-P+2
	\end{equation*}

	\begin{equation*}
		\left(\dfrac{\partial \mu}{\partial T}\right)_p=-S_m
	\end{equation*}

	\begin{equation*}
		\left(\dfrac{\partial \mu}{\partial p}\right)_T=V_m
	\end{equation*}

	\begin{equation*}
		\Delta S_{mix} = -nR\left(\chi_A\ln\chi_A+\chi_B\ln\chi_B\right)
	\end{equation*}

	\begin{equation*}
		p_B=\chi_BK_B
	\end{equation*}

	\begin{equation*}
		K_b=\frac{RT^{\star 2}_b}{\Delta H_{vap}}
	\end{equation*}
\end{minipage}

\noindent
\begin{minipage}[t]{0.5\linewidth}
	\begin{equation*}
		\Delta T_b=K_b\chi_B = K_bC_B
	\end{equation*}

	\begin{equation*}
		\Delta T_f=K_f\chi_B=K_fC_B
	\end{equation*}

	\begin{equation*}
		\frac{n_l}{n_{total}}=\left|\frac{z_B-y_B}{x_B-y_B}\right|
	\end{equation*}

	\begin{equation*}
		\mu_B=\mu^{\std}_B+RT\ln\gamma_B\chi_B
	\end{equation*}

	\begin{equation*}
		\log\gamma_\pm = -\frac{A\abs{z_+z_-}\sqrt{I}}{1+B\sqrt{I}} + CI
	\end{equation*}

	\begin{equation*}
		\Delta G = \Delta G^{\std} +RT\ln Q
	\end{equation*}

	\begin{equation*}
		\Delta G^{\std}=-RT\ln K_{eq}
	\end{equation*}

	\begin{equation*}
		K_p=K_C\left(RT\right)^{\Delta n}
	\end{equation*}

	\begin{equation*}
		E_{cell}=E^{\std}_{cell}-\frac{RT}{\nu F}\ln Q
	\end{equation*}
\end{minipage}
\begin{minipage}[t]{0.5\linewidth}
	\begin{equation*}
		K_f=\frac{RT^{\star 2}_f}{\Delta H_{freeze}}
	\end{equation*}

	\begin{equation*}
		\frac{n_g}{n_{total}}=\abs{\frac{x_B-z_B}{x_B-y_B}}
	\end{equation*}

	\begin{equation*}
		\ln\gamma_A=\xi\chi_B^2 \hspace{2em} \ln\gamma_B=\xi\chi_A^2
	\end{equation*}

	\begin{equation*}
		I = \frac{1}{2}\sum\limits_{ions}z_i^2\left(\frac{c_i}{c^{\std}}\right) \hspace{2em} c^{\std}=1~molal
	\end{equation*}

	\begin{equation*}
		\ln\frac{K_2}{K_1} = -\frac{\Delta H^{\std}}{R}\left(\frac{1}{T_2}-\frac{1}{T_1}\right)
	\end{equation*}

	\begin{equation*}
		E_{cell}=E_{cathode}-E_{anode}
	\end{equation*}

	\begin{equation*}
		\frac{\mathrm{d}E^{\std}_{cell}}{\mathrm{d}T}=\frac{\Delta S^{\std}}{\nu F}
	\end{equation*}

	\begin{equation*}
		\nu_CE^{\std}_C = \nu_AE^{\std}_A + \nu_BE^{\std}_B
	\end{equation*}

	\begin{equation*}
		\Delta H^{\std}=-\nu F\left(E^{\std}_{cell}-T\frac{\mathrm{d}E^{\std}_{cell}}{\mathrm{d}T}\right)
	\end{equation*}
\end{minipage}

\begin{equation*}
	J_{matter}=-D\frac{\mathrm{d}\mathcal{N}}{\mathrm{d}z} \hspace{6em} J_{energy}=-\kappa\frac{\mathrm{d}T}{\mathrm{d}z} \hspace{6em} J_{x-momentum}=-\eta\frac{\mathrm{d}v_x}{\mathrm{d}z}
\end{equation*}

\noindent
\begin{minipage}[t]{0.5\linewidth}
	\begin{equation*}
		D=\frac{1}{3}\lambda v_{mean}=\frac{1}{3}\left(\frac{k_BT}{\sigma p}\right)\left(\frac{8RT}{\pi M}\right)^{\nicefrac{1}{2}}
	\end{equation*}
\end{minipage}
\begin{minipage}[t]{0.5\linewidth}
	\begin{equation*}
		\eta = \frac{1}{3}\lambda v_{mean}m\mathcal{N}=\frac{pMD}{RT}
	\end{equation*}
\end{minipage}

\noindent
\begin{minipage}[t]{0.5\linewidth}
	\begin{equation*}
		\eta=\eta_0e^{\nicefrac{E_a}{RT}}
	\end{equation*}

	\begin{equation*}
		G=\frac{1}{R}=\kappa\frac{A}{l}
	\end{equation*}
\end{minipage}
\begin{minipage}[t]{0.5\linewidth}
	\begin{equation*}
		\kappa = \frac{1}{3} \lambda v_{mean}\nu\mathcal{N}k_B =  \frac{\nu pD}{T} \hspace{2em} \nu=\frac{1}{2}N_{D.o.F.}
	\end{equation*}

	\begin{equation*}
		\Lambda_m = \frac{\kappa}{c}=\left(z_+u_+\nu_++z_-u_-\nu_-\right)F
	\end{equation*}
\end{minipage}

\begin{equation*}
	f=6\pi\eta a \hspace{10em} u = \frac{ze}{f} \hspace{10em} s=uE=u\frac{\Delta V}{m}
\end{equation*}

\begin{equation*}
	c(x,t)=\frac{n_0}{A\sqrt{\pi Dt}}e^{-\nicefrac{x^2}{4Dt}} \hspace{10em} x_{rms}=\sqrt{2Dt}
\end{equation*}

\noindent
\begin{minipage}[t]{0.5\linewidth}
	\begin{equation*}
		v = \frac{\mathrm{d}\left[\ch{A}\right]}{\nu_A\mathrm{d}t}=\dfrac{1}{V}\dfrac{\mathrm{d}\xi}{\mathrm{d}t}
	\end{equation*}

	\begin{equation*}
		\chi = \chi_0e^{-\nicefrac{t}{\tau}}
	\end{equation*}

	\begin{equation*}
		k = Ae^{-\frac{E_a}{RT}}
	\end{equation*}

	\begin{equation*}
		v_{\mathrm{Lind.-Hinsh.}} = \dfrac{k_ak_b[A]^2}{k_b+k^\prime_a[A]}
	\end{equation*}

	\begin{equation*}
		\phi_{F,0}=\dfrac{k_F}{k_F+k_{IC}+k_{ISC}}= k_F\tau
	\end{equation*}

	\begin{equation*}
		\eta_T = 1 - \dfrac{\phi_F}{\phi_{F,0}} = \dfrac{R_0^6}{R_0^6 + R^6}
	\end{equation*}

	\begin{equation*}
		v= P\sigma v_{rel}N_A^2e^{-\frac{E_a}{RT}}[A][B]
	\end{equation*}


	\begin{equation*}
		k\propto e^{\nicefrac{\Delta S^{\ddagger}}{R}}e^{\nicefrac{\Delta H^{\ddagger}}{RT}}
	\end{equation*}
\end{minipage}
\begin{minipage}[t]{0.5\linewidth}
	\begin{equation*}
		\ln\left(\frac{v_2}{v_1}\right)=m\ln\left(\frac{\left[\ch{A}\right]_2}{\left[\ch{A}\right]_1}\right)
	\end{equation*}

	\begin{equation*}
		\tau = \dfrac{1}{k_r + k_r^\prime}
	\end{equation*}

	\begin{equation*}
		\ln\left(\frac{k_2}{k_1}\right)=-\frac{E_a}{R}\left(\frac{1}{T_2}-\frac{1}{T_1}\right)
	\end{equation*}

	\begin{equation*}
		\tau_0=\dfrac{1}{k_F+k_{IC}+k_{ISC}}
	\end{equation*}

	\begin{equation*}
		\dfrac{\phi_{0}}{\phi} = 1 + \tau_0k_Q[Q]
	\end{equation*}

	\begin{equation*}
		\frac{1}{v}=\frac{1}{v_{max}}+\left(\frac{K_M}{v_{max}}\right)\frac{1}{\left[\ch{S}\right]_0}
	\end{equation*}

	\begin{equation*}
		k_d=\dfrac{8RT}{3\eta}
	\end{equation*}
\end{minipage}

\end{document}
